backend/AliasAnalysisConclusion.v
@@ -1,0 +1,373 @@
+Require Import Relations.
+
+Require Import AST.
+Require Import Coqlib.
+Require Import Integers.
+Require Import Memory.
+Require Import Registers.
+Require Import RTL.
+Require Import Values.
+
+Require Import AliasAnalysis.
+Require Import AliasHierarchy.
+Require Import AliasLib.
+
+Definition disjoint (x y: PTSet.t) :=
+  forall a b, PTSet.In a x -> PTSet.In b y -> ~ AbsPO.overlap a b.
+
+Theorem disjoint_implies: forall
+  ge cs f sp pc rs m
+  (AI: alias_interprets ge (State cs f sp pc rs m))
+  rmap mmap (RES: (safe_funanalysis f)#pc = (rmap, mmap))
+  r1 r2 (DISJ: disjoint (RegMap.get r1 rmap) (RegMap.get r2 rmap))
+  b1 o1 (R1: rs # r1 = Vptr b1 o1)
+  b2 o2 (R2: rs # r2 = Vptr b2 o2)
+  ,
+  Vptr b1 o1 <> Vptr b2 o2.
+Proof.
+  repeat intro. inv H. destruct AI as [abs SAT]. inv SAT. inv RES0. rewrite RPC in RES. inv RES.
+  pose proof (RSAT r1) as Sr1. pose proof (RSAT r2) as Sr2.
+  unfold regsat, valsat in Sr1, Sr2.
+  rewrite R1 in Sr1. rewrite R2 in Sr2.
+  destruct (abs b2).
+  elim (DISJ (Loc a o2) (Loc a o2)); auto. apply reflexivity.
+  elim (DISJ AbsPH.top AbsPH.top); auto using PTSet.In_top. apply reflexivity.
+Qed.
+
+Definition disjoint_dec_bool (a b: PTSet.t): bool :=
+  PTSet.AbsPSet.for_all
+  (fun x =>
+    PTSet.AbsPSet.for_all
+    (fun y =>
+      negb (AbsPO.overlap_dec x y)
+    )
+    b
+  )
+  a.
+
+Module Facts := OverlapFacts(AbsPO).
+
+Theorem disjoint_dec_bool_spec: forall a b,
+  disjoint_dec_bool a b = true -> disjoint a b.
+Proof.
+  intros a b DISJ x y INx INy OVER.
+  apply PTSet.F.for_all_iff in DISJ.
+  apply PTSet.In_spec in INx; destruct INx as [INx | [ax [Ax INax]]].
+  Case "x is really in a".
+  specialize (DISJ x INx). simpl in DISJ.
+  apply PTSet.In_spec in INy; destruct INy as [INy | [ay [Ay INay]]].
+  SCase "y is really in b".
+  apply PTSet.F.for_all_iff in DISJ; auto.
+  specialize (DISJ y INy). simpl in DISJ.
+  destruct (AbsPO.overlap_dec x y). inv DISJ. contradiction.
+  repeat intro. subst. reflexivity.
+  SCase "y has an ancestor in b".
+  apply PTSet.F.for_all_iff in DISJ; auto.
+  specialize (DISJ ay INay). simpl in DISJ.
+  destruct (AbsPO.overlap_dec x ay). inv DISJ. elim n.
+  symmetry. eapply Facts.above_overlaps_too; eauto. now symmetry.
+  repeat intro. subst. reflexivity.
+  Case "x has an ancestor in a".
+  specialize (DISJ ax INax). simpl in DISJ.
+  apply PTSet.In_spec in INy; destruct INy as [INy | [ay [Ay INay]]].
+  SCase "y is really in b".
+  apply PTSet.F.for_all_iff in DISJ; auto.
+  specialize (DISJ y INy). simpl in DISJ.
+  destruct (AbsPO.overlap_dec ax y). inv DISJ.
+  elim n. eapply Facts.above_overlaps_too; eauto.
+  repeat intro. subst. reflexivity.
+  SCase "y has an ancestor in b".
+  apply PTSet.F.for_all_iff in DISJ; auto.
+  specialize (DISJ ay INay). simpl in DISJ.
+  destruct (AbsPO.overlap_dec ax ay). inv DISJ. elim n.
+  eapply Facts.above_overlaps_too; eauto. symmetry.
+  eapply Facts.above_overlaps_too; eauto. now symmetry.
+  repeat intro. subst. reflexivity.
+  repeat intro. subst. reflexivity.
+Qed.
+
+Definition disjoint_chunks (chunk1 chunk2: memory_chunk) (s1 s2: PTSet.t) :=
+  forall (p1 p2: AbsPO.t),
+    PTSet.In p1 s1 -> PTSet.In p2 s2 ->
+    match p1, p2 with
+    | Loc b1 o1, Loc b2 o2 =>
+      (b1 <> b2 /\ ~ AbsPO.AbsBO.overlap b1 b2)
+      \/ (Int.unsigned o1 + size_chunk chunk1 <= Int.unsigned o2)
+      \/ (Int.unsigned o2 + size_chunk chunk2 <= Int.unsigned o1)
+    | Loc b1 _, Blk b2 | Blk b1, Loc b2 _ | Blk b1, Blk b2 =>
+      b1 <> b2
+      \/ ~ AbsPO.AbsBO.overlap b1 b2
+    end.
+
+Theorem disjoint_chunks_implies: forall
+  ge cs f sp pc rs m
+  (AI: alias_interprets ge (State cs f sp pc rs m))
+  rmap mmap (RES: (safe_funanalysis f)#pc = (rmap, mmap))
+  chunk1 chunk2 r1 r2 (DISJ: disjoint_chunks chunk1 chunk2 (RegMap.get r1 rmap) (RegMap.get r2 rmap))
+  b1 o1 (R1: rs # r1 = Vptr b1 o1)
+  b2 o2 (R2: rs # r2 = Vptr b2 o2)
+  ,
+  b1 <> b2
+  \/ (Int.unsigned o1 + size_chunk chunk1 <= Int.unsigned o2)
+  \/ (Int.unsigned o2 + size_chunk chunk2 <= Int.unsigned o1).
+Proof.
+  intros. destruct AI as [abs SAT]. inv SAT. inv RES0. rewrite RPC in RES. inv RES.
+  pose proof (RSAT r1) as Sr1. pose proof (RSAT r2) as Sr2.
+  unfold regsat, valsat in Sr1, Sr2.
+  rewrite R1 in Sr1. rewrite R2 in Sr2.
+  destruct (abs b2) as [ab2|]_eqn, (abs b1) as [ab1|]_eqn.
+  specialize (DISJ _ _ Sr1 Sr2). simpl in DISJ. intuition.
+  left. intro. subst. rewrite Heqo in Heqo0. inv Heqo0. now apply H0.
+  simpl in DISJ. left. intro. subst. rewrite Heqo in Heqo0. congruence.
+  simpl in DISJ. left. intro. subst. rewrite Heqo in Heqo0. congruence.
+  unfold disjoint_chunks in DISJ.
+  specialize (DISJ (Loc AbsPO.AbsBO.top o1) (Loc AbsPO.AbsBO.top o2)). simpl in DISJ.
+  feed_all DISJ.
+  apply Sr1. apply PTSet.In_top.
+  apply Sr2. apply PTSet.In_top.
+  intuition.
+Qed.
+
+Theorem disjoint_chunks_implies2: forall
+  ge cs f sp pc rs m
+  abs (SAT: satisfy ge abs (State cs f sp pc rs m))
+  rmap mmap (RES: (safe_funanalysis f)#pc = (rmap, mmap))
+  chunk1 chunk2 set1 set2 (DISJ: disjoint_chunks chunk1 chunk2 set1 set2)
+  b1 o1 b2 o2
+  (In1:
+    match abs b1 with
+    | Some ab1 => PTSet.In (Loc ab1 o1) set1
+    | None     => PTSet.ge set1 PTSet.top
+    end
+  )
+  (In2:
+    match abs b2 with
+    | Some ab2 => PTSet.In (Loc ab2 o2) set2
+    | None     => PTSet.ge set2 PTSet.top
+    end
+  )
+  ,
+  b1 <> b2
+  \/ (Int.unsigned o2 + size_chunk chunk2 <= Int.unsigned o1)
+  \/ (Int.unsigned o1 + size_chunk chunk1 <= Int.unsigned o2).
+Proof.
+  intros. inv SAT. inv RES0. rewrite RPC in RES. inv RES.
+  (*
+  pose proof (RSAT r1) as Sr1. pose proof (RSAT r2) as Sr2.
+  unfold regsat, valsat in Sr1, Sr2.
+  rewrite R1 in Sr1. rewrite R2 in Sr2.
+  *)
+  destruct (abs b2) as [ab2|]_eqn, (abs b1) as [ab1|]_eqn.
+  specialize (DISJ _ _ In1 In2). simpl in DISJ. intuition.
+  left. intro. subst. rewrite Heqo in Heqo0. inv Heqo0. now apply H0.
+  simpl in DISJ. left. intro. subst. rewrite Heqo in Heqo0. congruence.
+  simpl in DISJ. left. intro. subst. rewrite Heqo in Heqo0. congruence.
+  unfold disjoint_chunks in DISJ.
+  specialize (DISJ (Loc AbsPO.AbsBO.top o1) (Loc AbsPO.AbsBO.top o2)). simpl in DISJ.
+  feed_all DISJ.
+  apply In1. apply PTSet.In_top.
+  apply In2. apply PTSet.In_top.
+  intuition.
+Qed.
+
+Theorem disjoint_chunks_implies3: forall
+  ge cs f sp pc rs m
+  abs (SAT: satisfy ge abs (State cs f sp pc rs m))
+  rmap mmap (RES: (safe_funanalysis f)#pc = (rmap, mmap))
+  chunk1 chunk2 set1 set2 (DISJ: disjoint_chunks chunk1 chunk2 set1 set2)
+  b o1 o2
+  (In1:
+    match abs b with
+    | Some ab => PTSet.In (Loc ab o1) set1 /\ PTSet.In (Loc ab o2) set2
+    | None    => PTSet.ge set1 PTSet.top /\ PTSet.ge set2 PTSet.top
+    end
+  )
+  ,
+  (Int.unsigned o2 + size_chunk chunk2 <= Int.unsigned o1)
+  \/ (Int.unsigned o1 + size_chunk chunk1 <= Int.unsigned o2).
+Proof.
+  intros.
+  pose proof (disjoint_chunks_implies2 _ _ _ _ _ _ _ _ SAT _ _ RES _ _ _ _ DISJ b o1 b o2).
+  feed_all H; destruct (abs b); intuition.
+Qed.
+
+(* Should be moved in Integers.v *)
+Theorem int_add_sub: forall a b,
+  Int.add (Int.sub a b) b = a.
+Proof.
+  intros. rewrite Int.sub_add_opp. rewrite Int.add_assoc.
+  setoid_rewrite Int.add_commut at 2. rewrite Int.add_neg_zero. now rewrite Int.add_zero.
+Qed.
+
+Theorem disjoint_chunks_shift_implies: forall
+  ge cs f sp pc rs m
+  (AI: alias_interprets ge (State cs f sp pc rs m))
+  rmap mmap (RES: (safe_funanalysis f)#pc = (rmap, mmap))
+  chunk1 chunk2 r1 r2 s1 s2
+  (DISJ: disjoint_chunks chunk1 chunk2
+    (shift_offset (RegMap.get r1 rmap) s1)
+    (shift_offset (RegMap.get r2 rmap) s2)
+  )
+  b1 o1 (R1: rs # r1 = Vptr b1 o1)
+  b2 o2 (R2: rs # r2 = Vptr b2 o2)
+  ,
+  (
+    b1 <> b2
+    \/ (Int.unsigned (Int.add o1 s1) + size_chunk chunk1 <= Int.unsigned (Int.add o2 s2))
+    \/ (Int.unsigned (Int.add o2 s2) + size_chunk chunk2 <= Int.unsigned (Int.add o1 s1))
+  )
+  \/
+  (
+    b1 <> b2
+    \/ (Int.unsigned o1 + size_chunk chunk1 <= Int.unsigned o2)
+    \/ (Int.unsigned o2 + size_chunk chunk2 <= Int.unsigned o1)
+  ).
+
+Proof.
+  intros. destruct AI as [abs SAT]. inv SAT. inv RES0. rewrite RPC in RES. inv RES.
+  pose proof (RSAT r1) as Sr1. pose proof (RSAT r2) as Sr2.
+  unfold regsat, valsat in Sr1, Sr2.
+  rewrite R1 in Sr1. rewrite R2 in Sr2.
+  destruct (abs b2) as [ab2|]_eqn, (abs b1) as [ab1|]_eqn.
+  eapply In_shift_offset with (o' := Int.add o1 s1) in Sr1; [|reflexivity].
+  eapply In_shift_offset with (o' := Int.add o2 s2) in Sr2; [|reflexivity].
+  specialize (DISJ _ _ Sr1 Sr2). simpl in DISJ. intuition.
+  left. left. intro. subst. rewrite Heqo in Heqo0. inv Heqo0. now apply H0.
+  left. simpl in DISJ. left. intro. subst. rewrite Heqo in Heqo0. congruence.
+  left. simpl in DISJ. left. intro. subst. rewrite Heqo in Heqo0. congruence.
+  right. unfold disjoint_chunks in DISJ.
+  specialize (DISJ (Loc AbsPO.AbsBO.top o1) (Loc AbsPO.AbsBO.top o2)). simpl in DISJ.
+  feed_all DISJ.
+  apply In_shift_offset with (o := Int.sub o1 s1). apply Sr1. apply PTSet.In_top.
+  auto using int_add_sub.
+  apply In_shift_offset with (o := Int.sub o2 s2). apply Sr2. apply PTSet.In_top.
+  auto using int_add_sub.
+  intuition.
+Qed.
+
+Definition disjoint_chunks_dec_bool chunk1 chunk2 (s1 s2: PTSet.t): bool :=
+  PTSet.AbsPSet.for_all
+  (fun p1 =>
+    PTSet.AbsPSet.for_all
+    (fun p2 =>
+      match p1, p2 with
+      | Loc b1 o1, Loc b2 o2 =>
+        ((negb (AbsPO.AbsBO.eq_dec b1 b2)) && (negb (AbsPO.AbsBO.overlap_dec b1 b2)))
+        || Int.no_overlap o1 (size_chunk chunk1) o2 (size_chunk chunk2)
+      | Loc b1 _, Blk b2 | Blk b1, Loc b2 _ | Blk b1, Blk b2 =>
+        ((negb (AbsPO.AbsBO.eq_dec b1 b2)) && (negb (AbsPO.AbsBO.overlap_dec b1 b2)))
+      end
+    )
+    s2
+  )
+  s1.
+
+Module AbsPHFacts := HierarchyFacts(AbsPH).
+
+Lemma above_blk: forall x z,
+  AbsPH.above (Blk x) (Blk z) ->
+  AbsPO.AbsBO.above x z.
+Proof.
+  unfold AbsPH.above, AbsPO.AbsBO.above. intros x.
+  setoid_rewrite clos_trans_tn1_iff.
+  refine (AbsPO.AbsBO.above_ind _ _); intros z IND H.
+  inv H.
+  left.
+  destruct x, z; try destruct a0; try destruct o; compute in *; congruence.
+  destruct y.
+  right with (y := t).
+  destruct t, z; try destruct a0; try destruct o; compute in *; try congruence.
+  apply IND; auto. apply AbsPO.AbsBO.parent_is_above.
+  destruct t, z; try destruct a0; try destruct o; compute in *; try congruence.
+  destruct t, z; try destruct a0; try destruct o; compute in *; try congruence.
+Qed.
+
+Lemma above_blk_loc: forall x z o,
+  AbsPH.above (Blk x) (Loc z o) ->
+  x = z \/ AbsPO.AbsBO.above x z.
+Proof.
+  unfold AbsPH.above, AbsPO.AbsBO.above. intros x.
+  setoid_rewrite clos_trans_tn1_iff.
+  refine (AbsPO.AbsBO.above_ind _ _); intros z o IND H.
+  inv H.
+  left.
+  destruct x, z; try destruct a0; try destruct o; compute in *; congruence.
+  destruct y.
+  assert (t = z).
+  destruct t, z; try destruct a0; try destruct o; compute in *; congruence.
+  subst.
+  assert (AbsPH.above (Blk x) (Blk z)).
+  unfold AbsPH.above. now setoid_rewrite clos_trans_tn1_iff.
+  apply above_blk in H. right.
+  unfold AbsPO.AbsBO.above in H. now setoid_rewrite clos_trans_tn1_iff in H.
+  exfalso.
+  destruct t, z; try destruct a0; try destruct o; compute in *; try congruence.
+Qed.
+
+Module AbsBOFacts := OverlapFacts(AbsPO.AbsBO).
+
+Ltac solver :=
+  repeat (intuition (idtac;
+    match goal with
+    | |- _ \/ _ => left
+    | |- _ \/ _ => right
+    | |- _ <> _ => intro
+
+    | H: AbsPH.above (Loc _ _) _ |- _ => apply not_loc_above in H
+    | H: AbsPH.above (Blk ?b) (Blk ?c) |- _ => apply above_blk in H
+    | H: AbsPH.above (Blk ?b) (Loc ?c ?o) |- _ => apply above_blk_loc in H
+
+    | _: _ = _ |- _ => progress subst
+    | _: _ = _ |- _ => discriminate
+    | H: ?x = ?x |- _ => clear H
+    | |- _ => AbsBOFacts.solver
+    | |- _ => fail
+    end
+  )).
+
+Theorem disjoint_chunks_dec_bool_spec: forall chunk1 chunk2 s1 s2,
+  disjoint_chunks_dec_bool chunk1 chunk2 s1 s2 = true -> disjoint_chunks chunk1 chunk2 s1 s2.
+Proof.
+  intros ???? DISJ x y INx INy.
+  apply PTSet.F.for_all_iff in DISJ; [|repeat intro; now subst].
+  apply PTSet.In_spec in INx; destruct INx as [INx | [ax [Ax INax]]].
+  Case "x is really in a".
+  specialize (DISJ x INx). simpl in DISJ.
+  apply PTSet.In_spec in INy; destruct INy as [INy | [ay [Ay INay]]].
+  SCase "y is really in b".
+  apply PTSet.F.for_all_iff in DISJ; [|repeat intro; now subst].
+  specialize (DISJ y INy). simpl in DISJ.
+  destruct x, y;
+  destruct (AbsPO.AbsBO.eq_dec t t0), (AbsPO.AbsBO.overlap_dec t t0);
+  simpl in DISJ; try solve [solver];
+  right;
+  apply Int.no_overlap_sound with (base := Int.zero) in DISJ; auto using size_chunk_pos;
+  simpl in DISJ;
+  setoid_rewrite Zmod_small in DISJ; auto using Int.unsigned_range.
+  SCase "y has an ancestor in b".
+  apply PTSet.F.for_all_iff in DISJ; [|repeat intro; now subst].
+  specialize (DISJ ay INay). simpl in DISJ.
+  destruct ay as [bay|? ?]; [|elim (not_loc_above _ _ _ Ay)].
+  destruct x as [bx|bx ox], y as [byy|byy oy];
+  destruct (AbsPO.AbsBO.eq_dec bx bay), (AbsPO.AbsBO.overlap_dec bx bay);
+  simpl in DISJ; solve [solver].
+  Case "x has an ancestor in a".
+  specialize (DISJ ax INax). simpl in DISJ.
+  apply PTSet.In_spec in INy; destruct INy as [INy | [ay [Ay INay]]].
+  SCase "y is really in b".
+  apply PTSet.F.for_all_iff in DISJ; [|repeat intro; now subst].
+  specialize (DISJ y INy). simpl in DISJ.
+  destruct ax as [bax|? ?]; [|elim (not_loc_above _ _ _ Ax)].
+  destruct x as [bx|bx ox], y as [byy|byy oy];
+  destruct (AbsPO.AbsBO.eq_dec bax byy), (AbsPO.AbsBO.overlap_dec bax byy);
+  simpl in DISJ; solve [solver].
+  SCase "y has an ancestor in b".
+  apply PTSet.F.for_all_iff in DISJ; [|repeat intro; now subst].
+  specialize (DISJ ay INay). simpl in DISJ.
+  destruct ax as [bax|? ?]; [|elim (not_loc_above _ _ _ Ax)].
+  destruct ay as [bay|bay oay];
+  destruct (AbsPO.AbsBO.eq_dec bax bay), (AbsPO.AbsBO.overlap_dec bax bay);
+  simpl in DISJ; try solve [solver];
+  destruct x as [bx|bx ox], y as [byy|byy oy];
+  solve [solver].
+Qed.
